add separators to imatch, some fancy syntax

coq/splitting/imatch.v
@@ -17,6 +17,8 @@ From Local Require Import splitting_tactics splitting_ltac2_tactics.
 Inductive not_false :=.
 (* where "⫫" := not_false. *)
 
+Inductive sep :=.
+
 From Ltac2 Require Import Ltac2.
 From Ltac2 Require Pattern Option.
 From Local Require utils.
@@ -35,7 +37,6 @@ end.
 
 Ltac2 Type iris_id := constr.
 Ltac2 Type iris_prop := constr.
-Ltac2 Type ('a, 'b) sum := [Left ('a) | Right ('b)].
 
 Ltac2 i_match_term (kpat : kinded_pattern) (term : constr) :=
   let (k, pat) := kpat in
@@ -59,34 +60,44 @@ Ltac2 rec pick_match_rec
       (acc : (iris_id * iris_prop) list)
       (env : (iris_id * iris_prop) list)
       (kpat : kinded_pattern)
-  := match env with
+  :=let bogus := '(1) in (* placeholder constr *)
+    match env with
     | [] => Control.zero IMatch_failure
     | eh :: et =>
       let (id, prop) := eh in
       let constraint := Std.eval_red '(fst $id) in
       let ident := Std.eval_red '(snd $id) in
-      Control.plus
-        (fun () =>
-           let (binders, ctxs) :=
-               match (Control.case (fun () => i_match_term kpat '(1, $prop))) with
-               | Err _ =>
-                 (* pattern for boolean constraint isn't a wildcard
-                    which means it might be not_false, so we should check
-                    that first *)
-                 or (fun () =>
-                       let (b,c) := i_match_term kpat '(not_false, $prop) in
-                       let is_false := Constr.equal (Std.eval_vm None constraint)
-                                                    '(false) in
-                       match is_false with
-                       | true => Control.zero (IMatch_failure)
-                       | false => (b,c)
-                       end)
-                    (fun () => i_match_term kpat '($constraint, $prop))
-               | Val _ => (* pattern for boolean constraint is a wildcard *)
-                 i_match_term kpat '($constraint, $prop)
-               end in
-             (ident, binders, ctxs, List.append (List.rev acc) et))
-          (fun _ => pick_match_rec (eh :: acc) et kpat)
+      List.fold_left
+        (fun x y () => Control.plus x y)
+        [
+         (** * First try to match just the PROP *)
+         (fun _ => let (bins, ctxs) := i_match_term kpat prop in
+                (ident, bins, ctxs, List.append (List.rev acc) et));
+         (** * Then try to match both the constraint and the prop *)
+         (fun _ =>
+            let (bins, ctxs) :=
+                match (Control.case
+                         (fun () => i_match_term kpat '($bogus, $prop))) with
+                | Err _ =>
+                  (* pattern for boolean constraint isn't a wildcard
+                 which means it might be not_false,
+                 so we should check that first *)
+                  or (fun () =>
+                        let (b,c) := i_match_term kpat '(not_false, $prop) in
+                        let is_false := Constr.equal (Std.eval_vm None constraint)
+                                                     '(false) in
+                        match is_false with
+                        | true => Control.zero (IMatch_failure)
+                        | false => (b,c)
+                        end)
+                     (fun () => i_match_term kpat '($constraint, $prop))
+                | Val _ =>
+                  (* pattern for boolean constraint is a wildcard *)
+                  i_match_term kpat '($constraint, $prop)
+                end in (ident, bins, ctxs, List.append (List.rev acc) et));
+         (** * Last thing - don't use this hypothesis at all *)
+         (fun _ => pick_match_rec (eh :: acc) et kpat)]
+        (fun () => Control.zero IMatch_failure) ()
     end.
 
 Ltac2 pick_match (env : (iris_id * iris_prop) list) (kpat : kinded_pattern) :=
@@ -94,37 +105,83 @@ Ltac2 pick_match (env : (iris_id * iris_prop) list) (kpat : kinded_pattern) :=
 
 Ltac2 rec i_match_ihyps_list
       (pats : kinded_patterns)
-      (penv : (iris_id * iris_prop) list)
-      (senv : (iris_id * iris_prop) list)
+      (env : (iris_id * iris_prop) list)
   := match pats with
-    | [] => ([], [], [])
-    | p :: pats' =>
-      let (i, b, c, e) :=
+     | [] => ([],[],[])
+     | p :: pats' =>
+       let (i, b, c, env') := pick_match env p in
+       let (it, bt, ct) := i_match_ihyps_list pats' env' in
+       (i:: it, b :: bt, c :: ct)
+     end.
+
+Ltac2 Type ('a, 'b, 'c) trisum := [First ('a) | Second ('b) | Third ('c)].
+
+Ltac2 split_pat_list_with_sep plist :=
+  let bogus := '(1) in (* placeholder constr *)
+  let rec go acc rest :=
+      match rest with
+      | [] => acc
+      | rh :: restl =>
+        let isnt_sep () := match acc with
+          | First a =>
+            go (First (rh :: a)) restl
+          | Second ab =>
+            let (a, b) := ab in
+            go (Second (rh :: a, b)) restl
+          | Third abc =>
+            let (a,b,c) := abc in
+            go (Third (rh :: a, b, c)) restl
+          end in
+        (* match against bogus term to find out whether the pattern is wildcard *)
+        match (Control.case (fun () => i_match_term rh bogus)) with
+        | Val _ =>
+          (* The pattern is a wildcard, so it's not sep *)
+          isnt_sep ()
+        | Err _ =>
+          (* The pattern is not a wildcard *)
           or (fun () =>
-                let (i, b, c, penv') := pick_match penv p in
-                (i, b, c , Left penv'))
-             (fun () =>
-                let (i, b, c, senv') := pick_match senv p in
-                (i, b, c, Right senv')) in
-      let (it, bt, ct) := match e with
-        | Left penv' => i_match_ihyps_list pats' penv' senv
-        | Right senv' => i_match_ihyps_list pats' penv senv'
-        end in
-      (i:: it, b :: bt, c :: ct)
-   end.
+                i_match_term rh '(sep);
+                (* if we get here, then previous expr didn't fail,
+                   so the rh pattern _is_ sep
+                   then we drop it and start a new partition in acc *)
+                match acc with
+                | First a => go (Second ([], a)) restl
+                | Second ab => let (a, b) := ab in go (Third ([], a, b)) restl
+                | Third abc => iriception "more than two separators in iMatch"
+                end)
+             (fun e => isnt_sep ())
+        end
+      end in
+  go (First []) (List.rev plist).
 
 Ltac2 i_match_ihyps
       (pats : kinded_patterns)
       (penv : constr)
       (senv : constr)
-  := let penvl := env_to_list penv in
-    let senvl := env_to_list senv in
-    let (ids, bins, ctxs) := i_match_ihyps_list pats penvl senvl in
-    let bins' := List.flat_map (fun x => to_list x) bins in
-    let ctxs' := List.flat_map (Option.map_default (fun e => [e]) []) ctxs in
-    (of_list ids '(1),
-     of_list bins' '(1),
-     of_list ctxs' (Pattern.empty_context())).
+  := let bogus := '(1) in (* placeholder constr *)
+     let penvl := env_to_list penv in
+     let senvl := env_to_list senv in
+     let (ids, bins, ctxs) :=
+         match (split_pat_list_with_sep pats) with
+         | First pats =>
+           i_match_ihyps_list pats (List.append penvl senvl)
+         | Second split_pats =>
+           let (ppats, spats) := split_pats in
+           let (ids1, bins1, ctxs1) :=
+             i_match_ihyps_list ppats penvl in
+           let (ids2, bins2, ctxs2) :=
+             i_match_ihyps_list spats senvl in
+           (List.append ids1 ('(sep) :: ids2),
+            List.append bins1 bins2,
+            List.append ctxs1 (None :: ctxs2))
+         | Third lll =>
+           iriception "Not implemented"
+         end in
+     let bins' := List.flat_map (fun x => to_list x) bins in
+     let ctxs' := List.flat_map (Option.map_default (fun e => [e]) []) ctxs in
+     (of_list ids   bogus,
+      of_list bins' bogus,
+      of_list ctxs' (Pattern.empty_context())).
 
 Ltac2 i_match_igoal conclpat concl :=
   let (knd, pat) := conclpat in
@@ -140,7 +197,7 @@ Ltac2 i_match_igoal conclpat concl :=
 
 Ltac2 i_matches_goal phyps pconcl :=
   lazy_match! goal with
-  | [|- @envs_entails ?pr1 (@Envs ?pr2 ?p ?s ?c) ?q] =>
+  | [|- envs_entails (Envs ?p ?s ?c) ?q] =>
     let (hids, hsubst, hctx) := i_match_ihyps phyps p s in
     let (gsubst, gctx) := i_match_igoal pconcl q in
     let hsubstl := to_list hsubst in
@@ -148,6 +205,23 @@ Ltac2 i_matches_goal phyps pconcl :=
     (hids, hctx, of_list (List.append hsubstl gsubstl) '(1), gctx)
   | [|- _] => Control.zero (Tactic_failure (Some (os "The goal isn't of the right shape")))
   end.
+
+Ltac2 i_lazy_match_goal pats :=
+  let rec interp m := match m with
+  | [] => Control.zero Match_failure
+  | p :: mt =>
+    let next _ := interp mt in
+    let (pat, f) := p in
+    let (phyps, pconcl) := pat in
+    let cur _ :=
+          let (hids, hctx, subst, cctx) := i_matches_goal phyps pconcl in
+          fun () => f hids hctx subst cctx
+    in Control.plus cur next
+  end in
+  Control.once (fun () => interp pats) ().
+
+Ltac2 Notation "iLazyMatch!" "goal" "with" m(goal_matching) "end" :=
+  i_lazy_match_goal m.
 
 Ltac2 i_match_goal pats :=
   let rec interp m := match m with
@@ -164,32 +238,32 @@ Ltac2 i_match_goal pats :=
   interp pats.
 
 Ltac2 i_match_one_goal pats := Control.once (fun _ => i_match_goal pats).
-
 Ltac2 Notation "iMatch!" "goal" "with" m(goal_matching) "end" :=
   i_match_one_goal m.
 
 From iris.proofmode Require Import classes notation.
 From Local Require Import ltac2_tactics.
-
 Context {PROP : sbi}.
 Implicit Types P Q R : PROP.
 
 Set Ltac2 Backtrace.
 
-Notation "'⟨' c '⟩' P" := (c%bool, P%I) (at level 10, c at level 0).
+Notation "'<' c '>' P" := (c%bool, P%I) (at level 10, c at level 0, only parsing).
+Notation "'<?>' P" := (not_false, P%I) (at level 10, only parsing).
+Notation "‖" := sep (only parsing).
 
-Lemma test_iAssumption_coq_1 P Q : Q ⊢ <affine> P -∗ Q.
+Lemma test1 P Q : Q ⊢ □ (<absorb> P) -∗ Q.
 Proof.
   i_start_split_proof ().
   i_intro_ident '(INamed "q").
-  i_intro_ident '(INamed "p").
-  iMatch! goal with
-  | [h1 : ⟨not_false⟩(<affine> _), h2 : _ |- ?p] => Message.print (oc h1)
+  (* i_intro_ident '(INamed "p").*)
+  i_intro_intuitionistic_ident '(INamed "p").
+  iLazyMatch! goal with
+  | [h2: (<absorb> _)%I, sep : ‖, h1 : <?> Q |- ?p] => Message.print (oc h2)
   end.
 
   iMatch! goal with
-  | [h1 : _, h2 : ⟨not_false⟩(<affine> _) |- ?p] =>
-    i_clear_hyp h2;
-    i_exact_spatial h1
+  | [h1 : _, h2 : <?> (<absorb> _) |- ?p] =>
+    i_clear_hyp h2; i_exact_spatial h1
   end.
 Qed.
